Smt translation: Bug fix for issues 194 and 195 + consider Array to encode HOF/Lambda terms

Tests/FixedIssues/Issue16.lean
@@ -4,6 +4,9 @@ import Blaster
 -- Issue: Valid result when counterexample expected
 -- Diagnosis : The use of Array type to model higher order function introduces unsound smt context.
 --             We therefore introduces ArrowTx types with the necessary congruences constraints.
+-- New Diagnosis : The theorems were wrongly formulated. Indeed, we can derive `false` from the hypothesis
+--                 by providing (λ _ => 0) as instance for `f`.
+--                 Use of Array type to represent HOF is sound provided that the isFun predicate is properly defined.
 
 namespace Tests.Issue16
 
@@ -21,20 +24,60 @@ mutual
 
 end
 
-#blaster (gen-cex: 0) (solve-result: 1)
-       [ (∀ (x : Int) (f : Int → Nat), f x > 2) →
-         (∀  (x y : Int) (f : Int → Nat), f x + f y > 20)
-       ]
+def example_1 :=
+  (∀ (x : Int) (f : Int → Nat), f x > 2) →
+  (∀  (x y : Int) (f : Int → Nat), f x + f y > 10)
 
-#blaster (gen-cex:0) (solve-result: 1)
-       [ (∀ (β : Type) (x : Term (List β)) (f : Term (List β) → Nat), f x > 0) →
-         (∀ (α : Type) (x y : Term (List α)) (f : Term (List α) → Nat), f x + f y > 20)
-       ]
+/-- Can be proved due to false hypothesis -/
+example : example_1 := by
+  simp [example_1]
+  intro h1 x y
+  have h2 := h1 x (λ _ => 0)
+  simp at h2
 
-#blaster (gen-cex:0) (solve-result: 1)
-       [ (∀ (β : Type) (x : Term (List β)) (g : Term (List β) → Nat), g x > 10) →
-         (∀ (α : Type) (x y : Term (List α)) (f : Term (List α) → Nat), f x + f y > 30)
-       ]
+-- Valid expected by Blaster
+#blaster [example_1]
 
+
+def example_2 :=
+  (∀ (β : Type) (x : Term (List β)) (f : Term (List β) → Nat), f x > 0) →
+  (∀ (α : Type) (x y : Term (List α)) (f : Term (List α) → Nat), f x + f y > 20)
+
+/-- Can be proved due to false hypothesis -/
+example : example_2 := by
+  simp [example_2]
+  intro h1 α x y
+  have h2 := h1 α x (λ _ => 0)
+  simp at h2
+
+-- Valid expected by Blaster
+#blaster [example_2]
+
+def example_3 :=
+  (∀ (β : Type) (x : Term (List β)) (g : Term (List β) → Nat), g x > 10) →
+  (∀ (α : Type) (x y : Term (List α)) (f : Term (List α) → Nat), f x + f y > 30)
+
+
+example : example_3 := by
+  simp [example_3]
+  intro h1 α x y
+  have h2 := h1 α x (λ _ => 0)
+  simp at h2
+
+-- Valid expected by Blaster
+#blaster [example_3]
+
+def example_4 :=
+  ∀ (f : Int → Nat), (∀ (x : Int), f x > 2) →
+  ∀ (x y : Int), f x + f y > 10
+
+#blaster (gen-cex: 0) (solve-result: 1) [example_4]
+
+def example_5 :=
+  ∀ (β : Type) (f : Term (List β) → Nat),
+   (∀ (x : Term (List β)), f x > 0) →
+   ∀ (x y : Term (List β)), f x + f y > 20
+
+#blaster (gen-cex: 0) (solve-result: 1) [example_5]
 
 end Tests.Issue16
