Tests/FixedIssues.lean
@@ -35,6 +35,8 @@ import Tests.FixedIssues.Issue35
 import Tests.FixedIssues.Issue36
 import Tests.FixedIssues.Issue143
 import Tests.FixedIssues.Issue152
+import Tests.FixedIssues.Issue194
+import Tests.FixedIssues.Issue195
 import Tests.FixedIssues.Issue227
 import Tests.FixedIssues.Issue262
 
